rocq/theories/TypeSystem/TypeSafetyClosureWrappersRuntimeArgs.v
@@ -5,6 +5,32 @@ From Facet.TypeSystem Require Export TypeSafetyClosureWrappersCleanup.
 From Stdlib Require Import List Bool ZArith String Program.Equality.
 Import ListNotations.
 
+Lemma apply_lt_params_nil_wrappers_runtime_args_ts :
+  forall ps,
+    apply_lt_params [] ps = ps.
+Proof.
+  intros ps.
+  induction ps as [| p ps IH].
+  - reflexivity.
+  - destruct p as [m x T].
+    unfold apply_lt_params in *.
+    simpl in *.
+    unfold apply_lt_param in *.
+    simpl in *.
+    change
+      ({| param_mutability := m; param_name := x;
+           param_ty := apply_lt_ty [] T |}
+        :: map
+             (fun p : param =>
+                {| param_mutability := param_mutability p;
+                   param_name := param_name p;
+                   param_ty := apply_lt_ty [] (param_ty p) |}) ps =
+       {| param_mutability := m; param_name := x; param_ty := T |} :: ps).
+    rewrite apply_lt_ty_nil_ts.
+    rewrite IH.
+    reflexivity.
+Qed.
+
 Lemma eval_make_closure_captured_call_runtime_args_ready_auto :
   forall env Ω n R Σ args fname captures captured fdef fcall used'
       s s_args vs R_args Σ_args arg_roots captured_tys,
@@ -98,12 +124,20 @@ Lemma eval_let_make_closure_captured_call_runtime_args_ready_auto :
       (call_param_root_env (fn_params fcall) arg_roots
         (empty_root_env_for_store captured ++ root_env_add x [] R_args)).
 Proof.
+  intros env Ω n R Σ args fname captures captured fdef fcall used'
+    s s_args_hidden s_args vs R_args Σ_args arg_roots captured_tys x T
+    Hstore Hroots Hshadow Hrn Hnamed Hkeys Hlookup Hcopy Hhidden
+    Heval_args Hrename Hcheck Hnodup_caps Hready_args Htyped_args
+    Hfresh_s Hfresh_captured.
   eapply
     (eval_let_make_closure_captured_call_runtime_args_ready_auto_with_preservation_core
       eval_preserves_typing_ready_mutual
       (eval_preserves_roots_ready_mutual_statement_to_package
         eval_preserves_roots_ready_mutual)
       eval_preserves_root_names_ready_mutual
-      eval_preserves_root_keys_named_ready_mutual);
+      eval_preserves_root_keys_named_ready_mutual
+      env Ω n R Σ args fname captures captured fdef fcall used' []
+      s s_args_hidden s_args vs R_args Σ_args arg_roots captured_tys x T);
+    try (rewrite apply_lt_params_nil_wrappers_runtime_args_ts);
     eassumption.
 Qed.
